rename cfg_collect_paths_

src/CFG/Collecting/CFG_Collecting_Core.thy
@@ -2,23 +2,23 @@ theory CFG_Collecting_Core
   imports CFG_Edges_Collect
 begin
 
-(* cfg_edges_collect and path-to-lfp bridge lemmas (pre-compound). *)
+(* cfg_collect_paths and path-to-lfp bridge lemmas (pre-compound). *)
 
 (* Path-based collecting environment. *)
-definition cfg_edges_collect :: "cfg => store set => pp => store set" where
-  "cfg_edges_collect g S v =
+definition cfg_collect_paths :: "cfg => store set => pp => store set" where
+  "cfg_collect_paths g S v =
      (\<Union>es\<in>{es. g \<turnstile> (cfg_entry g) \<longrightarrow>\<^bsub>es\<^esub> v}. edges_collect es S)"
 
 (* One CFG step extends path-based collecting. *)
-lemma cfg_edges_collect_step:
+lemma cfg_collect_paths_step:
   assumes e: "(u, a, v) : edges g"
-  shows "edge_collect a (cfg_edges_collect g S u) \<subseteq> cfg_edges_collect g S v"
+  shows "edge_collect a (cfg_collect_paths g S u) \<subseteq> cfg_collect_paths g S v"
 proof
   fix x
-  assume x: "x \<in> edge_collect a (cfg_edges_collect g S u)"
+  assume x: "x \<in> edge_collect a (cfg_collect_paths g S u)"
   then obtain es where es: "g \<turnstile> (cfg_entry g) \<longrightarrow>\<^bsub>es\<^esub> u"
     and x: "x \<in> edge_collect a (edges_collect es S)"
-    unfolding cfg_edges_collect_def
+    unfolding cfg_collect_paths_def
     by (smt (verit, ccfv_threshold) UN_iff edge_collect_member mem_Collect_eq)
   then obtain s where s: "s \<in> edges_collect es S"
     and x: "x \<in> edge_collect a {s}"
@@ -32,36 +32,36 @@ proof
     using x s unfolding edges_collect_append edges_collect.simps
     using edge_collect_member by blast 
  
-  then show "x \<in> cfg_edges_collect g S v"
-    unfolding cfg_edges_collect_def using es' by auto
+  then show "x \<in> cfg_collect_paths g S v"
+    unfolding cfg_collect_paths_def using es' by auto
 qed
 
-lemma cfg_edges_collect_entry:
-  "S \<subseteq> cfg_edges_collect g S (cfg_entry g)"
-  unfolding cfg_edges_collect_def by(auto)
+lemma cfg_collect_paths_entry:
+  "S \<subseteq> cfg_collect_paths g S (cfg_entry g)"
+  unfolding cfg_collect_paths_def by(auto)
  
 (*
-  Post-fixpoint: cfg_edges_collect satisfies cfg_collect_F.
+  Post-fixpoint: cfg_collect_paths satisfies cfg_collect_F.
   Proof via edges_collect_append + cfg_path_append; one line per edge action.
 *)
-lemma cfg_edges_collect_post:
-  "cfg_collect_F g S (cfg_edges_collect g S) v \<subseteq> cfg_edges_collect g S v"
+lemma cfg_collect_paths_post:
+  "cfg_collect_F g S (cfg_collect_paths g S) v \<subseteq> cfg_collect_paths g S v"
 proof -
-  have entry: "(if v = cfg_entry g then S else {}) \<subseteq> cfg_edges_collect g S v"
-    using cfg_edges_collect_entry by auto
-  have step: "collect_pp g (cfg_edges_collect g S) v \<subseteq> cfg_edges_collect g S v"
-    unfolding collect_pp_def using cfg_edges_collect_step by blast
+  have entry: "(if v = cfg_entry g then S else {}) \<subseteq> cfg_collect_paths g S v"
+    using cfg_collect_paths_entry by auto
+  have step: "collect_pp g (cfg_collect_paths g S) v \<subseteq> cfg_collect_paths g S v"
+    unfolding collect_pp_def using cfg_collect_paths_step by blast
   from entry step show ?thesis
     unfolding cfg_collect_F_def by blast
 qed
 
  
-lemma cfg_collect_le_edges_collect:
-  "cfg_collect g S v \<subseteq> cfg_edges_collect g S v"
+lemma cfg_collect_le_paths:
+  "cfg_collect g S v \<subseteq> cfg_collect_paths g S v"
 proof -
-  have pf: "cfg_collect_F g S (cfg_edges_collect g S) \<le> cfg_edges_collect g S"
-    unfolding le_fun_def using cfg_edges_collect_post by simp
-  have "lfp (cfg_collect_F g S) \<le> cfg_edges_collect g S"
+  have pf: "cfg_collect_F g S (cfg_collect_paths g S) \<le> cfg_collect_paths g S"
+    unfolding le_fun_def using cfg_collect_paths_post by simp
+  have "lfp (cfg_collect_F g S) \<le> cfg_collect_paths g S"
     using pf cfg_collect_F_mono lfp_lowerbound by blast
   then show ?thesis
     unfolding cfg_collect_def le_fun_def by simp
